@prefix cc: <http://creativecommons.org/ns#>.
@prefix skos: <http://www.w3.org/2004/02/skos/core#> .
@prefix rdf: <http://www.w3.org/1999/02/22-rdf-syntax-ns#> .
@prefix rdfs: <http://www.w3.org/2000/01/rdf-schema#> .
@prefix dc: <http://purl.org/dc/elements/1.1/>.
@prefix log: <http://www.w3.org/2000/10/swap/log#>.
@prefix owl: <http://www.w3.org/2002/07/owl#>.
@prefix vs: <http://www.w3.org/2003/06/sw-vocab-status/ns#> .
@prefix xsd: <http://www.w3.org/2001/XMLSchema#> .

<> a owl:Ontology ;
   rdfs:label "n3 definition of some Semantic Web terms";
   rdfs:comment """
These raise the level above RDF's pure relational data,
and Web Ontology's ontological level, to allow rules to be expressed
and inference done. They connect the inference to the web,
allowing data to be fetched from resources elsewhere, and remote
servers to be queried.
""";
   cc:license <http://www.w3.org/Consortium/Legal/copyright-software>;
   skos:historyNote """
n3 definition of some Semantic Web terms

These raise the level above RDF's pure relational data,
and Web Ontology's ontological level, to allow rules to be expressed
and inference done. They connect the inference to the web,
allowing data to be fetched from resources elsewhere, and remote
servers to be queried.

$Id: log.n3,v 1.25 2010-03-26 20:35:14 timbl Exp $
""".

log:N3Document a rdfs:Class;
    rdfs:label "N3Document";
    #rdfs:subClassOf doc:Work;
    rdfs:comment    """A document which, which parsed as Notation3
as defined in general by http://www.w3.org/DesignIssues/Notation3.html
and this schema, conveys the intent of the author by the semantics defined
on those specifications, and the semantics defined by the specifications
of any other identifiers used in the document.
""" .

################################################## Syntactic level
#
#  It isn't clear to me that these should be described as Properties
#  and Classes.  They operate at a level of symbol identity, not identity of the things referred to.
#

log:equalTo a rdf:Property, owl:FunctionalProperty, owl:InverseFunctionalProperty;
    rdfs:label "equalTo";
    rdfs:comment "True if the subject and object are the same RDF node (symbol or literal).";
    skos:note "Do not confuse with owl:sameAs.";
    skos:editorialNote "A cwm built-in logical operator, RDF graph level.";
    skos:example "";
    rdfs:isDefinedBy <>.

log:notEqualTo a rdf:Property;
    owl:inverse log:equalTo;
    rdfs:label "notEqualTo";
    rdfs:comment "Equality in this sense is actually the same URI.";
    skos:editorialNote "A cwm built-in logical operator.";
    skos:example "";
    rdfs:isDefinedBy <>.

log:rawType a rdf:Property, owl:FunctionalProperty;
    rdfs:label "rawType";
    rdfs:range log:Type;
    rdfs:comment "This is a low-level language type, one of log:Formula, log:Literal, log:List, log:Set or log:Other.";
    skos:note "log:semanticsOrError returns either a formula or a string, and you can check which using log:rawType.";
    skos:example "";
    rdfs:isDefinedBy <>.

log:Type a rdfs:Class;
    rdfs:label "Type";
    rdfs:comment "The class of Notation3-specifiec resource types.";
    vs:term_status "unstable";
    rdfs:isDefinedBy <>.

log:Formula a rdfs:Class; 
    rdfs:subClassOf log:Type;
    rdfs:label "Formula";
    rdfs:comment "The class of Notation-3 Formulae";
    rdfs:isDefinedBy <>.

log:List    a rdfs:Class; 
    rdfs:subClassOf log:Type, rdf:List;
    rdfs:label "List";
    rdfs:comment "A Notation-3 List, as a resource. A sub-class of an RDF List.";
    rdfs:isDefinedBy <>.

log:String  a rdfs:Class; 
    rdfs:subClassOf log:Type, rdfs:Literal;
    rdfs:label "List";
    rdfs:comment "An RDF Literal";
    rdfs:isDefinedBy <>.

log:Other   a rdfs:Class; 
    rdfs:subClassOf log:Type;
    rdfs:label "List";
    rdfs:comment "Some other Notation-3 type";
    rdfs:isDefinedBy <>.

#   The following are inherent in the translation of N3 syntax to quad representation:

# FIXME: no such thing as rdf:SyntaxArc.
log:forSome a rdf:SyntaxArc;  #@@@@@   NOT a real property. A pseudo property
    rdfs:label "for Some";
    rdfs:domain log:Formula;
    rdfs:comment """A is true for some object for which here we use B. This
is NOT a real rdf property in its behavior - a pseudo-property.
For example, removal of it from a formula does not
preserve truth, and substitution is not permitted on its object.""" ;
    vs:term_status "unstable";
    rdfs:isDefinedBy <>.

log:forAll a log:SyntaxArc;  #@@@@@   NOT a real property. A pseudo property
    rdfs:label     "for All";
    rdfs:domain log:Formula;
    rdfs:comment """A is true for any object in place of B.
This is NOT a real rdf property in its behavior - a pseudo-property.
For examples substitution is not permitted on its object.""";
    vs:term_status "unstable";
    rdfs:isDefinedBy <>.


#########################################################
#
#  The following are used for inference
#

log:Truth a rdfs:Class;
    rdfs:label "Truth";
    rdfs:comment "Something which is true: believe it as you would believe this.";
    skos:editorialNote "Understood natively by cwm in that it will execute rules in a formula declared a Truth within a formula it is already taking rules from.";
    rdfs:isDefinedBy <>.

#log:Falsehood a rdf:Class;
#   rdfs:label "Falsehood";
#   rdfs:comment "Something which is not true. Not the complement of True!";
#   rdfs:domain log:context.
#

log:implies a rdf:Property;
    rdfs:label "implies";
    rdfs:comment """Logical implication. 
This is the relation between the antecedent (subject) and
conclusion (object) of a rule.
The application of a rule to a knowledge-base is as follows.
For every substitution which, applied to the antecedent,
gives a formula which is a subset of the knowledge-base,
then the result of applying that same substitution to the
conclusion may be added to the knowledge-base.""";
    skos:editorialNote """related: See log:conclusion. 
(See the CWM manual for command line options to determine how
rules from different sources are applied to and the results
added to various formula.)""";
    skos:example "";
    rdfs:domain log:Formula;
    rdfs:range log:Formula;
    rdfs:isDefinedBy <>.

log:includes a rdf:Property;
    rdfs:label "includes";
    rdfs:comment """The subject formula includes the object formula.
Formula A includes formula B if there exists some substitution
which when applied to B creates a formula B' such that for
every statement in B' is also in A, every variable
universally (or existentially) quantified in B' is quantified in
the same way in A. 

Variable substitution is applied recursively to nested compound terms such as
formulae, lists and sets.""";
    skos:editorialNote """(Understood natively by cwm when in in the antecedent of a rule.
You can use this to peer inside nested formulae.)""";
    skos:example "";
    rdfs:domain log:Formula;
    rdfs:range log:Formula;
    rdfs:isDefinedBy <>.

log:notIncludes a rdf:Property;
    rdfs:label "not includes";
    rdfs:comment """The object formula is NOT a subset of subject.
True iff log:includes is false.
The converse of log:includes.""";
    skos:editorialNote """(Understood natively by cwm.
The subject formula may contain variables.
(In cwm, variables must of course end up getting bound
before the log:include test can be done, or an infinite result set
would result)
Related: See includes""";
    skos:example "";
    rdfs:domain log:Formula;
    rdfs:range log:Formula;
    rdfs:isDefinedBy <>.


# The following connect the inference engine to the web


log:parsedAsN3 a rdf:Property;
    rdfs:comment "The subject string, parsed as N3, gives this formula.";
    rdfs:label "parses to N3";
    skos:example "";
    rdfs:domain log:N3;
    rdfs:range log:Formula;
    rdfs:isDefinedBy <>.
 
 log:n3String a rdf:Property;
    rdfs:comment "The subject formula, expressed as N3, gives this string.";
    rdfs:label "n3 string";
    skos:example "";
    rdfs:domain log:Formula;
    rdfs:range log:N3;
    rdfs:isDefinedBy <>.

log:semantics a rdf:Property;
    #rdfs:domain doc:Work;
    rdfs:domain log:N3Document;
    rdfs:range  log:Formula;
    rdfs:label  "semantics";
    rdfs:comment """The log:semantics of a document is the formula.
achieved by parsing representation of the document.
For a document in Notation3, log:semantics is the
log:parsedAsN3 of the log:content of the document.
For a document in another RDF syntax, it is parsed according to the
appropriate specification to yield an RDF formula
(a subclass of N3 log:Formula).
Evaluates to false if an unrecognized document format is retrieved.

[Aside: Philosophers will be distracted here into worrying about the meaning
of meaning. At least we didn't call this function "meaning"!
In as much as N3 is used as an interlingua for interoperability
for different systems, this for an N3 based system is the meaning 
expressed by a document.]""";
    skos:example "";
    rdfs:isDefinedBy <>.

log:semanticsOrError a rdf:Property;
    #rdfs:domain doc:Work;
    rdfs:domain log:N3Document;
    rdfs:label  "semantics or error message";
    rdfs:comment """This connects a document and either the formula it parses to,
or an error message explaining what went wrong with trying. See log:semantics.""";
    skos:editorialNote "(Cwm knows how to go get a document and parse it in order to evaluate this.)" .

log:content a rdf:Property;
    #rdfs:domain doc:Work;
    rdfs:domain log:N3Document;
    rdfs:range  log:String;
    rdfs:label  "content";
    rdfs:comment "This connects a document and a string that represents it.";
    skos:editorialNote "(Cwm knows how to go get a document in order to evaluate this.)";
    skos:note "Note that the content-type of the information is not given and so must be known or guessed.";
    skos:example "";
    rdfs:isDefinedBy <>.

#  Merge two formulae

log:conjunction a rdf:Property;
    rdfs:label "conjunction";
    rdfs:domain log:List;
    rdfs:range  log:Formula;
    rdfs:comment """A function to merge formulae: logical AND.

The subject is a list of formulae.
The object, which can be generated, is a formula containing a copy
of each of the formulae in the list on the left.""";
    skos:editorialNote "A cwm built-in function.";
    skos:example "";
    rdfs:isDefinedBy <>.

#  Find the set of ALL statements entailed by a given formula.

log:conclusion a rdf:Property;
    rdfs:label "conclusion";
    rdfs:domain log:Formula;
    rdfs:range log:Formula;
    rdfs:comment """All possible conclusions which can be drawn from a formula.

The object of this function, a formula, is the set of conclusions which can be
drawn from the subject formula, by successively applying any
rules it contains to the data it contains.""";
    skos:editorialNote """This is equivalent to
cwm's "--think" command line function.  It does use built-ins, so
it may for example indirectly invoke other documents, validate
signatures, etc.""";
    skos:example "";
    rdfs:isDefinedBy <>.

############# Automatic processing steered by metadata

log:definitiveDocument a rdf:Property;
    rdfs:label "definitive document";
    rdfs:domain rdf:Property;
    #rdfs:range doc:Work;
    rdfs:range log:N3Document;
    rdfs:comment""" When document D is the definitiveDocument for property P,
any statement X P Y is true iff the semantics of document D
include that statement.""";
    skos:note """For example, there may be a definitive document for the zipcode of
airports by airport code, and so on. This is useful to let a reasoner
know that it can extend its query to the given document.""";
    skos:editorialNote "(Cwm will do this if its mode includes \"r\").";
    vs:term_status "deprecated";
    rdfs:isDefinedBy <>.

log:definitiveService a rdf:Property;
    rdfs:label "definitive service";
    rdfs:domain rdf:Property;
#   rdfs:range doc:Work;
    rdfs:comment """ When service S is the definitiveService for property P,
any statement X P Y is true iff and only if a query to S returns
that it is.  The protocol for the service S depends on the scheme.
For mysql protocol, the URI of the service is like
`sql://user:password@host.domain/database/`.""";
    skos:note """For example, there may be a definitive service for the zipcode of
airports by airport code, and so on. This is useful to let a reasoner
know that it can help resolve a query by delegating it to the service
in question.""";
    skos:editorialNote "(Cwm will do this if its mode includes \"r\").";
    vs:term_status "deprecated";
    rdfs:isDefinedBy <>.


################### String output

log:outputString a rdf:Property;
    rdfs:label "output string";
    rdfs:range log:String;
    rdfs:comment """The subject is a key and the object is a string,
where the strings are to be output in the order of the keys.""";
    skos:editorialNote "See cwm --strings in cwm --help.";
    vs:term_status "deprecated";
    rdfs:isDefinedBy <>.


################### Experimental

log:becomes a rdf:Property;
    rdfs:label "becomes";
    rdfs:comment "Built-in to perform RDF linear implication i.e. retracting the subject graph and asserting the object graph.";
    vs:term_status "unstable";
    rdfs:isDefinedBy <>.

log:dtlit a rdf:Property;
    rdfs:labe "dtlit";
    rdfs:domain log:List;
    rdfs:range rdfs:Literal;
    rdfs:comment "Takes a list of a string and a URI and creates a datatyped literal.";
    skos:example """`{ ("2005-03-30T11:00:00" :tz) log:dtlit ?X } => { ?X a :Answer } .`
will produce `"2005-03-30T11:00:00"^^:tz a :Answer .`""";
    vs:term_status "deprecated";
    rdfs:isDefinedBy <>.

log:findall a rdf:Property;
    rdfs:label "findall";
    rdfs:domain log:Formula;
    rdfs:range log:List;
    rdfs:comment """Built-in used as `?SCOPE e:findall (?SELECT ?WHERE ?ANSWER).`
Within the subject `?SCOPE` it unifies `?ANSWER` with a list that contains
all the instantiations of `?SELECT` satisfying the `?WHERE` clause.""";
    vs:term_status "unstable";
    rdfs:isDefinedBy <>.

log:forAllIn a rdf:Property;
    rdfs:label "forAllIn";
    rdfs:comment "Built-in for implementing a scoped universal quantification.";
    vs:term_status "unstable";
    rdfs:isDefinedBy <>.

log:forAllInClosure a rdf:Property;
    rdfs:label "forAllInClosure";
    rdfs:comment "Built-in for implementing a scoped universal quantification.";
    vs:term_status "unstable";
    rdfs:isDefinedBy <>.

log:notIn a rdf:Property;
    rdfs:label "notIn";
    rdfs:comment "Custom built-in for implementing scoped negation-as-failure (SNAF).";
    vs:term_status "unstable";
    rdfs:isDefinedBy <>.

log:notInClosure a rdf:Property;
    rdfs:label "notInClosure";
    rdfs:comment "Custom built-in for implementing scoped negation-as-failure (SNAF).";
    vs:term_status "unstable";
    rdfs:isDefinedBy <>.

log:skolem a rdf:Property;
    rdfs:label "skolem";
    rdfs:domain log:List;
    rdfs:range log:String;
    rdfs:comment "Built-in to generate a Skolem IRI object which is a function of the arguments in the subject list";
    vs:term_status "unstable";
    rdfs:isDefinedBy <>.

log:N3 a rdfs:Datatype;
    rdfs:subClassOf rdfs:Literal;
    rdfs:comment """The class log:N3 is the class of N3 literal values.
log:N3 is an instance of rdfs:Datatype and a subclass of rdfs:Literal.
The value of log:content of a log:N3Document is a literal with datatype log:N3.""";
    vs:term_status "unstable";
    rdfs:isDefinedBy <>.

################### Purge control

log:Chaff a rdfs:Class;
    rdfs:label "Chaff";
    rdfs:comment """Any statement mentioning anything in this class
is considered boring and purged by the cwm --purge option.
This is a convenience, and does not have any value when published as a
general fact on the web.""";
    rdfs:isDefinedBy <>.


################# Simple Builtins:
#

log:uri a rdf:Property;
    rdfs:lable "uri";
    rdfs:comment "This allows one to look at the actual string of the URI which identifies this.";
    skos:editorialNote "(Cwm can get the URI of a resource or get the resource from the URI.)";
    skos:note """This is a level breaker, breaking the rule of not looking inside a
URI.   Use (eg with  string:match) to replace RDF's old "aboutEach"
functionality. Use to implement the URI spec and protocol specs, etc.""";
    skos:example "";
    rdfs:range log:String;
    rdfs:isDefinedBy <>.

log:rawUri a rdf:Property;
    rdfs:label "raw uri";
    rdfs:comment "This allows one to look at the actual string of the URI which identifies this, for anything, even a blank node or a formula.";
    skos:editorialNote "This peeks into the internal workings of cwm, and so is not normally used. Use log:uri instead.";
    skos:example "";
    rdfs:range log:String;
    rdfs:isDefinedBy <>.

log:racine a rdf:Property;
    rdfs:label "racine";
    rdfs:comment """For anything identified by a URI with a fragid, this is the
thing identified by the same URI without a hash or fragid.
For anything else, it is itself.""";
    skos:example "";
    rdfs:isDefinedBy <>.

